testdata/export/shapes.cue
@@ -1,0 +1,9 @@
+emptyStruct: {}
+emptyList: []
+nestedList: [[], [1]]
+scalars: [1, 2, 3]
+maps: [{kind: "A", x: 1}, {kind: "B", y: 2}]
+block: """
+	line one
+	line two
+	"""
